coqimp/contextswitch/proof/TaskSwitchNewContext.v
@@ -1,0 +1,412 @@
+Require Import Coqlib.                                  
+Require Import Maps.            
+Require Import LibTactics.   
+        
+Require Import Integers.  
+Open Scope Z_scope.        
+Import ListNotations.  
+   
+Set Asymmetric Patterns.  
+        
+Require Import state.    
+Require Import language. 
+ 
+Set Implicit Arguments.    
+Unset Strict Implicit. 
+               
+Require Import logic.
+    
+Require Import lemmas.
+Require Import lemmas_ins.
+
+Require Import Coq.Logic.FunctionalExtensionality.
+
+Require Import integer_lemma.
+
+Require Import sep_lemma.
+Require Import reg_lemma.
+Require Import derived_rule.
+
+Require Import tm_dly_lemma.
+
+Require Import code.
+Require Import ctxswitch_spec.
+
+Require Import lemma1.
+
+Open Scope nat.
+Open Scope code_scope.
+Open Scope mem_scope.
+
+(*+ Lemmas for Integer +*)
+Lemma set_wim_eq_post_cwp :
+  forall id,
+    $ 0 <=ᵤᵢ id <=ᵤᵢ $ 7 ->
+    get_range 0 7 ((($ 1) <<ᵢ id) >>ᵢ ($ 7)) |ᵢ ((($ 1) <<ᵢ id) <<ᵢ ($ 1)) =
+                                              ($ 1) <<ᵢ (post_cwp id).
+Proof.
+  intros.
+  unfold get_range.
+  unfold post_cwp.
+  unfolds int_leu.
+  unfolds Int.ltu, Int.eq.
+  unfold Int.shl.
+  unfold Int.shru.
+  unfold Int.add.
+  unfold Int.sub.
+  unfold N.
+  simpl.
+  assert (Int.unsigned $ 0 = 0%Z).
+  eauto.
+  assert (Int.unsigned $ 1 = 1%Z).
+  eauto.
+  assert (Int.unsigned $ 7 = 7%Z).
+  eauto.
+  assert (Int.unsigned $ 8 = 8%Z).
+  eauto.
+  try rewrite H0 in *.
+  try rewrite H1 in *.
+  try rewrite H2 in *.
+  try rewrite H3 in *.
+  destruct id. 
+  simpls Int.unsigned.
+  unfold Int.modu, Int.or, Int.and.
+  rewrite H3.
+  destruct (zlt 0 intval); destruct (zeq 0 intval);
+    destruct (zlt intval 7); destruct (zeq intval 7);
+      tryfalse; try omega; eauto.
+  {
+    destruct intval; tryfalse.
+    do 3 (try destruct p; eauto; tryfalse).
+  }
+  {
+    subst; eauto.
+  }
+  {
+    subst; eauto.
+  }
+Qed.
+
+(*+ Lemmas for Space +*)
+
+(*+ Lemmas for Inference Rule +*)
+
+(*+ Proof +*)
+Theorem Ta0TaskSwitchNewContextProof :
+  forall vl,
+    spec |- {{ ta0_task_switch_newcontext_pre vl }}
+             ta0_task_switch_newcontext
+            {{ ta0_task_switch_newcontext_post vl }}.
+Proof.
+  intros.
+  unfold ta0_task_switch_newcontext_pre.
+  unfold ta0_task_switch_newcontext_post.
+  hoare_ex_intro_pre. 
+  renames x' to fmg, x'0 to fmo, x'1 to fml, x'2 to fmi.
+  renames x'3 to id, x'6 to vi, x'4 to F.
+  renames x'5 to vy, x'12 to vz, x'13 to vn.
+  renames x'8 to ct, x'9 to nt, x'7 to ll, x'10 to nctx, x'11 to nstk.
+  eapply Pure_intro_rule.
+  introv Hlgvl.
+  hoare_lift_pre 13.
+  eapply Pure_intro_rule.
+  introv Hnctx_addr_pt.
+  hoare_lift_pre 13.
+  eapply Pure_intro_rule.
+  introv Hid.
+  subst vi.
+
+  unfold ta0_task_switch_newcontext.
+  destruct fmg, fmo, fml, fmi.
+
+  hoare_lift_pre 2.
+  eapply backward_rule.
+  introv Hs.
+  eapply Regs_Global_combine_GenRegs in Hs; eauto.
+
+  (** set OSTaskNew l4 *)
+  eapply seq_rule.
+  TimReduce_simpl.
+  eapply set_rule_reg; eauto.
+  simpl upd_genreg.
+
+  (** ld [l4] l4 *)
+  hoare_lift_pre 7.
+  hoare_lift_pre 2.
+  eapply seq_rule.
+  TimReduce_simpl.
+  eapply ld_rule_reg; eauto.
+  simpl upd_genreg.
+
+  (** add l4 (OS_CONTEXT_OFFSET) l5 *)
+  eapply seq_rule.
+  TimReduce_simpl.
+  eapply add_rule_reg; eauto.
+  simpl; eauto.
+  unfold OS_CONTEXT_OFFSET.
+  rewrite in_range84; eauto.
+  simpl upd_genreg.
+
+  (** call reg_restore; nop *) 
+  eapply call_rule.
+  {
+    eval_spec.
+  }
+  {
+    TimReduce_simpl.
+    introv Hs.
+    eapply GenRegs_split_one with (rr := r15) in Hs.
+    simpls get_genreg_val'.
+    eauto.
+  }
+  {
+    TimReduce_simpl.
+    eapply nop_rule; eauto.
+  }
+  {
+    instantiate
+      (1 :=
+         logic_fm ([[w, w0, w1, w2, w3, w4, w5, w6]])
+          :: logic_fm ([[w7, w8, w9, w10, w11, w12, w13, $ 392]])
+          :: logic_fm ([[w15, w16, w17, w18, nt, nt +ᵢ ($ 84), w21, w22]])
+          :: logic_fm ([[w23, w24, w25, w26, w27, w28, w29, w30]])
+          :: logic_lv id :: logic_lv ((post_cwp id)) :: logic_fmls F :: logic_ctx nctx
+          :: logic_lv vy :: logic_lv ($ 392) :: nil
+      ).
+    unfold reg_restore_pre.
+    introv Hs.
+    sep_ex_elim_in Hs.
+    eapply sep_pure_l_elim in Hs.
+    destruct Hs as [Hlgvl1 Hs].
+    symmetry in Hlgvl1.
+    inversion Hlgvl1; subst. 
+    clear Hlgvl1.
+    simpl_sep_liftn_in Hs 5.
+    eapply sep_pure_l_elim in Hs.
+    destruct Hs as [Hpure Hs].
+    simpljoin1.
+    match goal with
+    | H : get_frame_nth _ 7 = Some _ |- _ =>
+      renames H to Hretf
+    end.
+    simpl in Hretf.
+    inversion Hretf; subst.
+    simpl.
+    destruct_state s.
+    simpl.
+    eapply getR_eq_get_genreg_val1 with (rr := r15) in Hs; eauto.
+  }
+  {
+    introv Hs.
+    eapply GenRegs_upd_combine_one in Hs; eauto.
+    simpls upd_genreg.
+    unfold reg_restore_pre.
+    sep_ex_intro.
+    asrt_to_line 5.
+    eapply sep_pure_l_intro; eauto.
+    sep_cancel1 1 1.
+    sep_cancel1 9 1.
+    sep_cancel1 3 1.
+    sep_cancel1 2 1.
+    eapply sep_pure_l_intro; eauto.
+    simpl.
+    repeat (split; eauto).
+    unfolds OS_CONTEXT_OFFSET.
+    simpljoin1; eauto.
+  }
+  {
+    eauto.
+  } 
+  {
+    introv Hs.
+    unfolds reg_restore_post.
+    sep_ex_elim_in Hs.
+    eapply sep_pure_l_elim in Hs.
+    destruct Hs as [Hlgvl1 Hs].
+    symmetry in Hlgvl1.
+    inversion Hlgvl1; subst.
+    clear Hlgvl1.
+    simpl.
+    destruct_state s.
+    simpl.
+    eapply getR_eq_get_genreg_val1 with (rr := r15) in Hs; eauto.
+  }
+  {
+    DlyFrameFree_elim.
+  }
+
+  unfold reg_restore_post.
+  hoare_ex_intro_pre.
+  eapply backward_rule.
+  introv Hs.
+  asrt_to_line_in Hs 5.
+  eauto.
+  eapply Pure_intro_rule.
+  introv Hlgvl1.
+  symmetry in Hlgvl1.
+  inversion Hlgvl1; subst.
+  clear Hlgvl1.
+
+  hoare_lift_pre 5.
+  eapply Pure_intro_rule.
+  introv Hctx_win_restore.
+  destruct Hctx_win_restore as [Hctx_win_restore Hretf].
+
+  (** set OSTaskSwitchFlag l4 *)
+  eapply seq_rule.
+  TimReduce_simpl.
+  eapply set_rule_reg; eauto.
+  simpl upd_genreg.
+
+  (** set OSFALSE l5 *)
+  eapply seq_rule.
+  TimReduce_simpl.
+  eapply set_rule_reg; eauto.
+  simpl upd_genreg.
+
+  (** st l5 [l4] *)
+  hoare_lift_pre 9.
+  hoare_lift_pre 2.
+  eapply seq_rule.
+  TimReduce_simpl.
+  eapply st_rule_reg; eauto.
+  simpl get_genreg_val.
+
+  (** set OSTaskCur l4 *)
+  eapply seq_rule.
+  TimReduce_simpl.
+  eapply set_rule_reg; eauto.
+  simpl upd_genreg.
+
+  (** set OSTaskNew l5 *)
+  eapply seq_rule.
+  TimReduce_simpl.
+  eapply set_rule_reg; eauto.
+  simpl upd_genreg.
+
+  (** ld [l5] l5 *)
+  hoare_lift_pre 6.
+  hoare_lift_pre 2.
+  eapply seq_rule.
+  TimReduce_simpl.
+  eapply ld_rule_reg; eauto.
+  simpl upd_genreg.
+
+  (** st l5 [l4] *)
+  hoare_lift_pre 9.
+  hoare_lift_pre 2.
+  eapply seq_rule.
+  TimReduce_simpl.
+  eapply st_rule_reg; eauto.
+  simpl get_genreg_val.
+
+  (** rd wim o4 *)
+  hoare_lift_pre 7.
+  hoare_lift_pre 2.
+  eapply seq_rule.
+  TimReduce_simpl.
+  eapply rd_rule_reg_wim; eauto.
+  simpl upd_genreg.
+
+  eapply hoare_pure_gen' with (pu := $ 0 <=ᵤᵢ id <=ᵤᵢ $ 7 /\ $ 0 <=ᵤᵢ (post_cwp id) <=ᵤᵢ $ 7).
+  {
+    introv Hs.
+    simpl_sep_liftn_in Hs 2.
+    unfold FrameState in Hs.
+    asrt_to_line_in Hs 3.
+    simpl_sep_liftn_in Hs 4.
+    eapply sep_pure_l_elim in Hs.
+    simpljoin1; eauto.
+  }
+  eapply Pure_intro_rule; eauto.
+  introv Hid_range.
+  destruct Hid_range as [Hid_range Hvi_range].
+
+  (** sll o4 1 o5 *)
+  eapply seq_rule.
+  TimReduce_simpl.
+  eapply sll_rule_reg; eauto.
+  simpls.
+  rewrite in_range1; eauto.
+  simpl upd_genreg.
+
+  (** srl o4 (OS_WINDOWS - 1) o5 *)
+  unfold OS_WINDOWS at 1.
+  assert (Heq7 : ($ 8) -ᵢ ($ 1) = ($ 7)); eauto.
+  rewrite Heq7.
+  eapply seq_rule.
+  TimReduce_simpl.
+  eapply srl_rule_reg; eauto.
+  simpl.
+  rewrite in_range7; eauto.
+  simpl upd_genreg. 
+  rewrite get_range_0_4_stable; eauto.
+  rewrite get_range_0_4_stable; eauto.
+
+  (** or o4 o5 o4 *)
+  eapply seq_rule.
+  TimReduce_simpl.
+  eapply or_rule_reg; eauto.
+  simpl; eauto.
+  simpl upd_genreg.
+
+  (** wr o4 0 wim *)
+  hoare_lift_pre 2.
+  eapply backward_rule.
+  introv Hs.
+  unfold FrameState in Hs.
+  asrt_to_line_in Hs 3.
+  simpl_sep_liftn_in Hs 2.
+  simpl_sep_liftn_in Hs 5.
+  eauto.
+  eapply seq_rule.
+  TimReduce_simpl.
+  eapply wr_rule_reg; eauto.
+  simpl.
+  rewrite in_range0; eauto.
+  simpl set_spec_reg.
+  rewrite Int.xor_zero; eauto.
+
+  (** nop *)
+  eapply seq_rule.
+  TimReduce_simpl.
+  eapply nop_rule; eauto.
+
+  (** nop *)
+  eapply seq_rule.
+  TimReduce_simpl.
+  eapply nop_rule; eauto.
+
+  (** nop *)
+  eapply seq_rule.
+  TimReduce_simpl.
+  eapply nop_rule; eauto.
+  rewrite set_wim_eq_post_cwp; eauto.
+
+  (** restore *)
+  eapply hoare_pure_gen' with (pu := length F = 13).
+  introv Hs.
+  simpl_sep_liftn_in Hs 4.
+  eapply sep_pure_l_elim in Hs; eauto.
+  simpljoin1; eauto.
+  eapply Pure_intro_rule.
+  introv Hlen_F.
+  destruct F; simpl in Hlen_F; tryfalse.
+  destruct F; simpl in Hlen_F; tryfalse.
+  destruct f, f0.
+  hoare_lift_pre 3.
+  hoare_lift_pre 3.
+  hoare_lift_pre 3.
+  eapply seq_rule.
+  TimReduce_simpl.
+  eapply restore_rule_reg; eauto.
+  simpl; eauto.
+  unfold win_masked.
+  destruct (((($ 1) <<ᵢ (post_cwp id)) &ᵢ (($ 1) <<ᵢ (post_cwp (post_cwp id)))) !=ᵢ ($ 0))
+           eqn:Heqe;
+    eauto.
+  Search Int.and.
+  
+  >>>>>>>>>>>>>>>>>>>>>>>>>>
+  
+  set_wim_eq_pre_cwp
